StateTransformer image is now an applicative.

src/StateTransformer.v
@@ -3,6 +3,8 @@ Add LoadPath "./" as Monads .
 Require Import Monads.FunctorApplicativeMonad.
 
 From Coq Require Import FunctionalExtensionality Program.Basics.
+Notation "x <- c1 ;; c2" := (bind c1 (fun x => c2)) 
+                             (right associativity, at level 84, c1 at next level).
 
 Set Universe Polymorphism.
 
@@ -35,12 +37,12 @@ Definition exec_state_t {m s a} `{Monad m} (r : state_t s m a) (x : s) : m s :=
 
 Definition state_map {m s} `{Monad m} {a b} (f : a -> b) (r : state_t s m a)
   : state_t s m b :=
-  fun (s0: s) => (bind (r s0) (fun (y:a*s) => pure(f (fst y), snd y))).
+  fun x => apply (map (fun y => (f (fst y), snd y))) (r x).
     
-Print state_map.
 
-Lemma fst_snd_in_monad {a s m} `{Monad m}: 
-(fun y : a * s => pure (fst y, snd y)) = (fun y : a * s => pure y).
+
+Lemma fst_snd_in_fun {a s m} `{Monad m}: 
+(fun y : a * s =>  (fst y, snd y)) = (fun y : a * s =>  y).
 Proof. apply functional_extensionality; intros; rewrite pair_fst_snd; trivial. Qed.
 
 Lemma state_functor_identity {m s a} `{Monad m} 
@@ -48,5 +50,130 @@ Lemma state_functor_identity {m s a} `{Monad m}
   : state_map id r = id r.
 
 Proof. unfold state_map. apply functional_extensionality. intros. unfold id.
-rewrite fst_snd_in_monad. apply bind_right_identity. Qed.
+rewrite fst_snd_in_fun. apply functor_identity. Qed.
+
+Lemma state_functor_composition_identity {m s a b c} `{Monad m} 
+  (u : b -> c) (v : a -> b) (r : state_t s m a)
+  : state_map (u <<< v) r = ((state_map u) <<< (state_map v)) r.
+Proof. unfold state_map. apply functional_extensionality. intros.
+change (fun y => ((u <<< v) (fst y), snd y))
+    with ((fun y => (v (fst y), snd y)) >>> (fun y : b * s => (u (fst y), snd y))).
+    apply functor_map_identity. Qed.
+
+#[program]
+Instance state_Functor (m :  Type -> Type) `{Monad m} (s : Type)
+  : Functor (state_t s m) :=
+  { map := @state_map m s _
+  }.
+
+Next Obligation.
+  apply state_functor_identity.
+Defined.
+
+Next Obligation.
+  apply state_functor_composition_identity.
+Defined.
+
+
+Definition state_apply {m s} `{Monad m} {a b}
+  (f : state_t s m (a -> b)) (fs : state_t s m a)
+  : state_t s m b :=
+  fun x => u <- f x ;; v <- fs (snd u);; pure (fst u (fst v), snd v).
+
+Definition state_pure {m s} `{Monad m} {a} (x : a) : state_t s m a :=
+  fun s => pure (x, s).
+
+Lemma state_applicative_identity {m s} `{Monad m} {a} (v : state_t s m a):
+  state_apply (state_pure id) v = v.
+Proof. unfold state_apply, state_pure. apply functional_extensionality. intros.
+rewrite bind_left_identity. simpl. unfold id. 
+assert (H1: (fun (v0:a*s) => pure (fst v0, snd v0))= (fun v0 =>pure  v0)).
+- apply functional_extensionality. intros. destruct x0; auto.
+- rewrite H1. apply bind_right_identity. Qed.
+
+Lemma state_applicative_homomorphism {m s} `{Monad m}{a b}
+  (v : a -> b) (x : a)
+  : state_apply (state_pure v) (state_pure x) = state_pure (m:=m) (s:=s) (v x).
+
+Proof. unfold state_pure, state_apply. apply functional_extensionality. intros.
+repeat rewrite bind_left_identity. auto. Qed.
+
+Lemma state_applicative_interchange {m s} `{Monad m} {a b}
+  (u : state_t s m (a -> b)) (y : a)
+  : state_apply u (state_pure y) = state_apply (state_pure (fun z : a -> b => z y)) u.
+Proof. unfold state_apply, state_pure. apply functional_extensionality. intros.
+rewrite bind_left_identity. 
+match goal with
+  | |- bind _ ?f = bind _ ?g =>
+    assert (R : f = g); [| now rewrite R ]
+  end. apply functional_extensionality. intros. rewrite bind_left_identity. auto. Qed.
+  
+#[program]
+Instance state_Applicative (m : Type -> Type) `{Monad m} (s : Type) 
+  : Applicative (state_t s m) :=
+  { pure := @state_pure m s _
+  ; apply := @state_apply m s _
+  }.
+  
+Next Obligation.
+  apply state_applicative_identity.
+Defined.
+
+Next Obligation.
+apply functional_extensionality. intros.
+  unfold state_apply, state_pure.
+  repeat rewrite bind_associativity.
+  repeat rewrite bind_left_identity.
+  repeat rewrite bind_associativity.
+  
+  match goal with
+  | |- bind _ ?f = bind _ ?g => assert (R: f = g); [| now rewrite R ]
+  end.
+  apply functional_extensionality. intros.
+  repeat rewrite bind_associativity.
+  repeat rewrite bind_left_identity.
+  repeat rewrite bind_associativity.
+  
+  match goal with
+  | |- bind _ ?f = bind _ ?g => assert (R: f = g); [| now rewrite R ]
+  end.
+  apply functional_extensionality. intros.
+
+  repeat rewrite bind_associativity.
+  repeat rewrite bind_left_identity.
+
+  match goal with
+  | |- bind _ ?f = bind _ ?g => assert (R: f = g); [| now rewrite R ]
+  end.
+ apply functional_extensionality. intros.
+
+  unfold compose.
+  repeat rewrite bind_left_identity.
+  cbn.
+  reflexivity.
+Defined.
+
+Next Obligation.
+  apply state_applicative_homomorphism.
+Defined.
+
+Next Obligation.
+   apply state_applicative_interchange.
+Defined.
+
+Lemma apply_map_bind_pure {m} `{Monad m} {a b}(x: m a) (f:a-> b): 
+apply (map f) x = bind x (fun t => pure (f t)).
+Proof. Admitted.
+
+
+
+Next Obligation.
+  unfold state_map, state_pure, state_apply.
+  apply functional_extensionality. intros.
+  rewrite bind_left_identity. 
+  cbn. apply apply_map_bind_pure. Defined.
+
+
+
+ 
  
